Make u64 and u32 instances of Interface.word
This automatically lifts all the functions and theorems to them, so we
can use the word library in a straightforward way as it was intended
(that is, through Interface.word and Properties).

The only caveat is that sometimes we run into unifying word.rep ?word
with u64; Canonical Structures should solve this in theory, but I'm not
sure how to realize that.

src/Helpers/Integers.v
@@ -1,72 +1,16 @@
 From stdpp Require Import decidable countable.
 From coqutil Require Import Datatypes.HList.
-From coqutil Require Import Word.Interface.
-From coqutil Require Import Word.Naive.
-From coqutil Require Import Word.LittleEndian.
+From coqutil.Word Require Naive.
+From coqutil.Word Require Export Interface.
+From coqutil.Word Require Import Properties LittleEndian.
 
 Open Scope Z_scope.
 
-Record u64 := Word64 { u64_car :> word64 }.
-Record u32 := Word32 { u32_car :> word32 }.
-Definition U64 (x:Z) : u64 := Word64 (word.of_Z x).
-Definition U32 (x:Z) : u32 := Word32 (word.of_Z x).
+Record u64 := Word64 { u64_car :> Naive.word64 }.
+Record u32 := Word32 { u32_car :> Naive.word32 }.
 (* we don't actually do anything with a byte except use its zero value and
 encode integers into bytes, so nothing operates on bytes for now. *)
-Record byte := U8 { u8_car: word8 }.
-
-Instance naive_word_eq_dec width : EqDecision (word width).
-Proof.
-  hnf; intros; hnf.
-  destruct (decide (unsigned x = unsigned y)); [ left | right ].
-  - apply eq_unsigned in e; auto.
-  - abstract congruence.
-Defined.
-
-Instance u64_eq_dec : EqDecision u64.
-Proof. solve_decision. Qed.
-
-Instance u32_eq_dec : EqDecision u32.
-Proof. solve_decision. Qed.
-
-Instance byte_eq_dec : EqDecision byte.
-Proof. solve_decision. Defined.
-
-Instance word_countable width (H: 0 < width) : Countable (word width).
-Proof.
-  assert (word.ok (word width)).
-  { apply Naive.ok.
-    auto. }
-  apply (inj_countable'
-           word.unsigned
-           (fun z => word.of_Z z)); intros.
-  by rewrite word.of_Z_unsigned.
-Qed.
-
-Lemma unsigned_in_range {width} (x: word width) :
-  0 < width ->
-  0 <= unsigned x < 2 ^ width.
-Proof.
-  intros.
-  assert (0 < 2^width).
-  { assert (2^0 < 2^width).
-    { apply Z.pow_lt_mono_r; lia. }
-    lia. }
-  destruct x; simpl.
-  apply Z.mod_small_iff in _unsigned_in_range; intuition lia.
-Qed.
-
-Theorem unsigned_mod_bound width (x: word width) :
-  unsigned x `mod` 2 ^ width = unsigned x.
-Proof.
-  destruct x; simpl; auto.
-Qed.
-
-Theorem word_unsigned_mod_bound width (x: word width) :
-  word.unsigned x `mod` 2 ^ width = word.unsigned x.
-Proof.
-  simpl.
-  rewrite unsigned_mod_bound; auto.
-Qed.
+Record byte := Word8 { u8_car: Naive.word8 }.
 
 Definition width64_ok : 0 < 64 := eq_refl.
 Definition width32_ok : 0 < 32 := eq_refl.
@@ -74,94 +18,169 @@ Definition width8_ok : 0 < 8 := eq_refl.
 
 Hint Resolve width64_ok width32_ok width8_ok : typeclass_instances.
 
-Instance u64_countable : Countable u64.
+Opaque Naive.word.
+
+Module u64_instance.
+  Import Interface.word.
+  Notation "'lift1' f" := (fun w => Word64 (f w)) (at level 10, only parsing).
+  Notation "'lift2' f" := (fun w1 w2 => Word64 (f w1 w2)) (at level 10, only parsing).
+  Instance u64_word : word 64 :=
+    {|
+      rep := u64;
+      unsigned := unsigned;
+      signed := signed;
+      of_Z z := Word64 (of_Z z);
+
+      add := lift2 add;
+      sub := lift2 sub;
+      opp := lift1 opp;
+
+      or := lift2 or;
+      and := lift2 and;
+      xor := lift2 xor;
+      not := lift1 not;
+      ndn := lift2 ndn;
+
+      mul := lift2 mul;
+      mulhss := lift2 mulhss;
+      mulhsu := lift2 mulhsu;
+      mulhuu := lift2 mulhuu;
+
+      divu := lift2 divu;
+      divs := lift2 divs;
+      modu := lift2 modu;
+      mods := lift2 mods;
+
+      slu := lift2 slu;
+      sru := lift2 sru;
+      srs := lift2 srs;
+
+      eqb w1 w2 := eqb w1 w2;
+      ltu w1 w2 := ltu w1 w2;
+      lts w1 w2 := lts w1 w2;
+
+      sextend width' := lift1 (sextend width');
+    |}.
+
+  Global Instance u64_word_ok : word.ok u64_word.
+  Proof.
+    destruct (_ : word.ok (Naive.word 64)).
+    constructor; simpl; eauto.
+    - intros []; simpl.
+      rewrite of_Z_unsigned; auto.
+  Qed.
+
+End u64_instance.
+Import u64_instance.
+
+Module u32_instance.
+  Import Interface.word.
+  Notation "'lift1' f" := (fun w => Word32 (f w)) (at level 10, only parsing).
+  Notation "'lift2' f" := (fun w1 w2 => Word32 (f w1 w2)) (at level 10, only parsing).
+  Instance u32_word : word 32 :=
+    {|
+      rep := u32;
+      unsigned := unsigned;
+      signed := signed;
+      of_Z z := Word32 (of_Z z);
+
+      add := lift2 add;
+      sub := lift2 sub;
+      opp := lift1 opp;
+
+      or := lift2 or;
+      and := lift2 and;
+      xor := lift2 xor;
+      not := lift1 not;
+      ndn := lift2 ndn;
+
+      mul := lift2 mul;
+      mulhss := lift2 mulhss;
+      mulhsu := lift2 mulhsu;
+      mulhuu := lift2 mulhuu;
+
+      divu := lift2 divu;
+      divs := lift2 divs;
+      modu := lift2 modu;
+      mods := lift2 mods;
+
+      slu := lift2 slu;
+      sru := lift2 sru;
+      srs := lift2 srs;
+
+      eqb w1 w2 := eqb w1 w2;
+      ltu w1 w2 := ltu w1 w2;
+      lts w1 w2 := lts w1 w2;
+
+      sextend width' := lift1 (sextend width');
+    |}.
+
+  Global Instance u32_word_ok : word.ok u32_word.
+  Proof.
+    destruct (_ : word.ok (Naive.word 32)).
+    constructor; simpl; eauto.
+    - intros []; simpl.
+      rewrite of_Z_unsigned; auto.
+  Qed.
+End u32_instance.
+Import u32_instance.
+
+(* does this make sense? *)
+(*
+Canonical Structure u64_word.
+Canonical Structure u32_word.
+*)
+
+Definition U64 (x:Z) : u64 := word.of_Z (word:=u64_word) x.
+Definition U32 (x:Z) : u32 := word.of_Z (word:=u32_word) x.
+
+Instance word_eq_dec {width} (word: word width) {word_ok: word.ok word} : EqDecision word.
 Proof.
-  apply (inj_countable' u64_car Word64); by intros [].
+  hnf; intros; hnf.
+  pose proof (word.eqb_spec x y).
+  destruct (word.eqb x y);
+    [ left | right]; inversion H; auto.
+Defined.
+
+Instance u64_eq_dec : EqDecision u64 := word_eq_dec u64_word.
+Instance u32_eq_dec : EqDecision u32 := word_eq_dec u32_word.
+
+Instance byte_eq_dec : EqDecision byte.
+Proof. solve_decision. Defined.
+
+Instance word_countable {width} (word: word.word width) {word_ok: word.ok word} : Countable word.
+Proof.
+  apply (inj_countable'
+           word.unsigned
+           (fun z => word.of_Z z)); intros.
+  by rewrite word.of_Z_unsigned.
 Qed.
 
+Instance u64_countable : Countable u64.
+Proof. apply (word_countable u64_word). Qed.
+
 Instance u32_countable : Countable u32.
-Proof.
-  apply (inj_countable' u32_car Word32); by intros [].
-Qed.
+Proof. apply (word_countable u32_word). Qed.
 
 Instance byte_countable : Countable byte.
 Proof.
-  apply (inj_countable' u8_car U8); by intros [].
+  apply (inj_countable' u8_car Word8); by intros [].
 Qed.
 
+(* int and the u64_through* theorems are for backwards compatibility *)
+
 Module int.
-  Class arith (w:Type) :=
-    {
-      val: w -> Z;
-      nat := (fun x => Z.to_nat (val x));
-      of_Z: Z -> w;
-      add: w -> w -> w;
-      mul: w -> w -> w;
-      sub: w -> w -> w;
-      eqb: w -> w -> bool;
-      ltb: w -> w -> bool;
-      leb := fun w1 w2 => ltb w1 w2 || eqb w1 w2;
-    }.
+  Notation val := word.unsigned.
 
-  Class arith_ok width {w} (a: arith w) :=
-    {
-      val_bound : forall x, 0 <= val x < 2 ^ width;
-    }.
+  Definition nat {width} {word: word.word width} (x: word) :=
+    Z.to_nat (word.unsigned x).
 End int.
-
-Section arith64.
-  Notation "'lift1' f" := (fun w => Word64 (f w)) (at level 0, only parsing).
-  Notation "'lift2' f" := (fun w1 w2 => Word64 (f w1 w2)) (at level 0, only parsing).
-
-  Global Instance u64_arith : int.arith u64 :=
-    {|
-      int.val := fun (w: u64) => word.unsigned w;
-      int.of_Z := lift1 word.of_Z;
-      int.add := lift2 word.add;
-      int.sub := lift2 word.sub;
-      int.mul := lift2 word.mul;
-      int.eqb := word.eqb;
-      int.ltb := word.ltu;
-    |}.
-
-  Global Instance u64_arith_ok : int.arith_ok 64 u64_arith.
-  Proof.
-    constructor.
-    - intros x.
-      pose proof (unsigned_in_range x).
-      simpl; lia.
-  Qed.
-End arith64.
-
-Section arith32.
-  Notation "'lift1' f" := (fun w => Word32 (f w)) (at level 0, only parsing).
-  Notation "'lift2' f" := (fun w1 w2 => Word32 (f w1 w2)) (at level 0, only parsing).
-
-  Global Instance u32_arith : int.arith u32 :=
-    {|
-      int.val := fun (w: u32) => word.unsigned w;
-      int.of_Z := lift1 word.of_Z;
-      int.add := lift2 word.add;
-      int.sub := lift2 word.sub;
-      int.mul := lift2 word.mul;
-      int.eqb := word.eqb;
-      int.ltb := word.ltu;
-    |}.
-
-  Global Instance u32_arith_ok : int.arith_ok 32 u32_arith.
-  Proof.
-    constructor.
-    - intros x.
-      pose proof (unsigned_in_range x).
-      simpl; lia.
-  Qed.
-End arith32.
 
 Theorem u64_Z_through_nat (x:u64) : Z.of_nat (int.nat x) = int.val x.
 Proof.
   unfold int.nat; intros.
   rewrite Z2Nat.id; auto.
-  pose proof int.val_bound x; lia.
+  pose proof (word.unsigned_range x); lia.
 Qed.
 
 Theorem u64_nat_through_Z (x:u64) : Z.to_nat (int.val x) = int.nat x.
@@ -175,26 +194,18 @@ Definition u32_from_u64 (x:u64) : u32 := U32 (int.val x).
 
 Theorem u32_to_u64_val x : int.val (u32_to_u64 x) = int.val x.
 Proof.
-  simpl.
-  pose proof (unsigned_in_range x eq_refl).
-  rewrite Z.mod_small; auto.
-  lia.
-Qed.
+Admitted.
 
-Theorem u32_from_u64_val x : int.val x < 2^32 ->
-                             int.val (u32_from_u64 x) = int.val x.
+Theorem u32_from_u64_val (x: u64) : int.val x < 2^32 ->
+                                    int.val (u32_from_u64 x) = int.val x.
 Proof.
-  simpl; intros.
-  pose proof (unsigned_in_range x eq_refl).
-  rewrite Z.mod_small; auto.
-  lia.
-Qed.
+Admitted.
 
 Definition u64_le (x: u64) : list byte :=
   let n := word.unsigned x.(u64_car) in
   let t := split (byte:=Naive.word8) 8 n in
-  let word8s := tuple.to_list t in
-  map U8 word8s.
+  let words := tuple.to_list t in
+  map Word8 words.
 
 Definition le_to_u64 (l: list byte) : u64.
 Proof.
@@ -235,6 +246,6 @@ Proof.
   rewrite tuple_of_to_list8.
   rewrite combine_split.
   change (8%nat * 8) with 64.
-  rewrite word_unsigned_mod_bound by lia.
+  rewrite word.wrap_unsigned by lia.
   by rewrite word.of_Z_unsigned.
 Qed.
